\begin{align*}
%
& %
% ['=', 'b', ['-', 'c', '1']]
b = c - 1
%
\land
%
% ['not', ['=', ['f', ['+', 'b', '1']], ['+', 'b', '2']]]
f(b + 1)  \neq  b + 2
%
\land
%
% ['=', ['select', 'A', ['f', 'c']], ['-', 'c', '1']]
\mathit{read}(A,f(c)) = c - 1
~\\~
& %
%
\land
%
% ['or', ['=', ['select', 'A', ['f', ['+', 'b', '1']]], ['+', 'b', '3']], ['=', ['select', ['store', 'A', ['+', 'b', '2'], ['f', ['-', 'c', '1']]], ['f', 'c']], ['+', 'c', '1']]]
(\mathit{read}(A,f(b + 1)) = b + 3 \lor \mathit{read}(\mathit{write}(A,b + 2,f(c - 1)),f(c)) = c + 1)
%
\end{align*}
