\begin{align*}
%
& %
% ['=', ['-', 'b', '2'], 'c']
b - 2 = c
%
\land
%
% ['not', ['=', ['f', ['-', 'b', '1']], 'b']]
f(b - 1)  \neq  b
%
\land
%
% ['=', ['select', 'A', ['f', ['+', 'c', '1']]], 'c']
\mathit{read}(A,f(c + 1)) = c
~\\~
& %
%
\land
%
% ['or', ['=', ['select', 'A', ['f', ['-', 'b', '1']]], ['+', 'b', '1']], ['=', ['select', ['store', 'A', 'b', ['f', 'c']], ['f', ['+', 'c', '1']]], ['+', 'c', '2']]]
(\mathit{read}(A,f(b - 1)) = b + 1 \lor \mathit{read}(\mathit{write}(A,b,f(c)),f(c + 1)) = c + 2)
%
\end{align*}
