\begin{align*}
%
& %
% ['=', ['-', 'b', '3'], ['+', 'c', '1']]
b - 3 = c + 1
%
\land
%
% ['not', ['=', ['f', ['-', 'b', '2']], ['-', 'b', '1']]]
f(b - 2)  \neq  b - 1
%
\land
%
% ['=', ['select', 'A', ['f', ['+', 'c', '2']]], ['+', 'c', '1']]
\mathit{read}(A,f(c + 2)) = c + 1
~\\~
& %
%
\land
%
% ['or', ['=', ['select', 'A', ['f', ['-', 'b', '2']]], 'b'], ['=', ['select', ['store', 'A', ['-', 'b', '1'], ['f', ['+', 'c', '1']]], ['f', ['+', 'c', '2']]], ['+', 'c', '3']]]
(\mathit{read}(A,f(b - 2)) = b \lor \mathit{read}(\mathit{write}(A,b - 1,f(c + 1)),f(c + 2)) = c + 3)
%
\end{align*}
